Prove termination of while loop, tidy

isabelle/Distinct_Elems_While.thy
@@ -9,18 +9,22 @@ begin
 context with_threshold
 begin
 
-definition fix_state_while :: \<open>'a state \<Rightarrow> 'a state spmf\<close> where
-  \<open>fix_state_while \<equiv> loop_spmf.while (\<lambda> state.
-    card (state_chi state) = threshold) (\<lambda> state. do {
-      let chi = state_chi state;
+definition cond :: \<open>'a state \<Rightarrow> bool\<close> where
+  \<open>cond \<equiv> \<lambda> state. card (state_chi state) = threshold\<close>
 
-      keep_in_chi :: 'a \<Rightarrow> bool \<leftarrow>
-        prod_pmf chi \<lblot>bernoulli_pmf <| 1 / 2\<rblot>;
+definition body :: \<open>'a state \<Rightarrow> 'a state pmf\<close> where
+ \<open>body \<equiv> \<lambda> state. do {
+  let chi = state_chi state;
 
-      let chi = Set.filter keep_in_chi chi;
-      let k = state_k state + 1;
+  keep_in_chi :: 'a \<Rightarrow> bool \<leftarrow>
+    prod_pmf chi \<lblot>bernoulli_pmf <| 1 / 2\<rblot>;
 
-      return_spmf \<lparr>state_k = k, state_chi = chi\<rparr>})\<close>
+  let chi = Set.filter keep_in_chi chi;
+  let k = state_k state + 1;
+
+  return_pmf \<lparr>state_k = k, state_chi = chi\<rparr>}\<close>
+
+abbreviation \<open>body_spmf \<equiv> spmf_of_pmf <<< body\<close>
 
 definition step_while :: \<open>'a \<Rightarrow> 'a state \<Rightarrow> 'a state spmf\<close> where
   \<open>step_while x state \<equiv> do {
@@ -32,7 +36,7 @@ definition step_while :: \<open>'a \<Rightarrow> 'a state \<Rightarrow> 'a state
         then insert x
         else Set.remove x);
 
-    fix_state_while (state\<lparr>state_chi := chi\<rparr>) }\<close>
+    loop_spmf.while cond body_spmf (state\<lparr>state_chi := chi\<rparr>) }\<close>
 
 definition estimate_distinct_while :: \<open>'a list \<Rightarrow> nat spmf\<close> where
   \<open>estimate_distinct_while \<equiv> run_steps_then_estimate_spmf step_while\<close>
@@ -41,7 +45,37 @@ end
 context with_threshold_pos
 begin
 
-lemma aux :
+lemma lossless_step_while_loop :
+  fixes state
+  defines [simp] : \<open>chi \<equiv> state_chi state\<close>
+  assumes \<open>finite chi\<close>
+  shows \<open>lossless_spmf <| loop_spmf.while cond body_spmf state\<close>
+proof -
+  have [simp] :
+    \<open>{keep_in_chi. card (Set.filter keep_in_chi chi) = card chi} =
+      chi \<rightarrow> {True}\<close>
+    if \<open>finite chi\<close> for chi :: \<open>'a set\<close>
+    using that
+    apply (intro set_eqI)
+    apply (simp add: Pi_iff)
+    by (metis card_mono card_seteq finite_filter member_filter subsetI)
+
+  from \<open>finite chi\<close> threshold_pos have [simp] :
+    \<open>pmf (map_pmf cond (body state)) True = 1 / 2 ^ threshold\<close>
+    if \<open>cond state\<close> for state :: \<open>'a state\<close>
+    using that
+    by (auto
+      simp add:
+        cond_def body_def Let_def vimage_def pmf_map field_simps card_ge_0_finite
+        map_pmf_def[symmetric] measure_Pi_pmf_Pi measure_pmf_single)
+
+  show ?thesis
+    by (auto
+      intro: loop_spmf.termination_0_1_immediate
+      simp add: pmf_False_conv_True threshold_pos)
+qed
+
+(* lemma aux :
   fixes state
   defines \<open>chi \<equiv> state_chi state\<close>
   assumes \<open>finite chi\<close> \<open>card chi \<le> threshold\<close>
@@ -61,7 +95,7 @@ lemma aux :
   apply (subst bind_spmf_of_pmf[symmetric])+
   apply (subst loop_spmf.while.simps)
   apply (subst bind_spmf_assoc)
-  using assms by simp
+  using assms by simp *)
 
 (* thm SPMF.fundamental_lemma[
   where p = \<open>spmf_of_pmf (step_no_fail x state)\<close>,
@@ -71,251 +105,6 @@ lemma aux :
     \<open>\<lambda> state'. card (state_chi state') \<ge> threshold\<close>
     (* \<open>\<lambda> state'. state_k state' > state_k state + 1\<close> *)
 ] *)
-
-text
-  \<open>If 2 probabilistic if-then-else expressions differ in only one branch of
-  computation, the total variation metric between their output distributions
-  is bounded by the probability that their guard condition evaluates such that
-  that branch of computation is taken.
-
-  This generalises and captures the essence behind bounding the distance between
-  running a while loop for only 1 iteration vs running it for \<ge> 1 iterations.
-
-  The proof of this result utilises the fundamental lemma for spmfs, along with
-  automation provided by our probabilistic relational Hoare logic for spmfs.\<close>
-lemma aux' :
-  fixes cond g and f f' :: \<open>'a \<Rightarrow> 'a spmf\<close>
-  assumes [simp] :
-    \<open>\<And> x. lossless_spmf (f x)\<close>
-    \<open>\<And> x. lossless_spmf (f' x)\<close>
-    \<open>\<And> x. lossless_spmf (g x)\<close>
-  defines [simp] : \<open>go \<equiv> \<lambda> f x. if cond x then f x else g x\<close>
-  notes [simp] = space_measure_spmf
-  shows
-    \<open>\<bar>\<P>(x in measure_spmf <| p \<bind> go f. P x)
-      - \<P>(x in measure_spmf <| p \<bind> go f'. P x)\<bar>
-    \<le> \<P>(x in measure_spmf p. cond x)\<close>
-    (is \<open>?L \<le> _\<close>)
-proof -
-  let ?kleisli_spmf_p = \<open>(>=>) \<lblot>p\<rblot>\<close>
-  let ?go_with_flag = \<open>\<lambda> f x.
-    if cond x
-    then pair_spmf (return_spmf True) (f x)
-    else pair_spmf (return_spmf False) (g x)\<close>
-
-  have \<open>?L =
-    \<bar>\<P>(x in measure_spmf <| p \<bind> ?go_with_flag f. P (snd x))
-      - \<P>(x in measure_spmf <| p \<bind> ?go_with_flag f'. P (snd x))\<bar>\<close>
-    apply (simp add:
-      if_distrib map_spmf_bind_spmf comp_def
-      measure_map_spmf[
-        of snd, where A = \<open>{x. P x}\<close>,
-        simplified vimage_def, simplified, symmetric])
-    unfolding map_snd_pair_spmf weight_return_spmf scale_spmf_1 ..
-
-  also have \<open>\<dots> \<le> \<P>(x in measure_spmf <| p \<bind> ?go_with_flag f. fst x)\<close>
-  proof -
-    have \<open>\<turnstile>spmf
-      \<lbrace>\<lblot>\<lblot>True\<rblot>\<rblot>\<rbrace>
-      \<langle>?kleisli_spmf_p (?go_with_flag f) | ?kleisli_spmf_p (?go_with_flag f')\<rangle>
-      \<lbrace>(\<lambda> (flag, y) (flag', y'). (flag \<longleftrightarrow> flag') \<and> (\<not> flag \<longrightarrow> y = y'))\<rbrace>\<close>
-      unfolding pair_spmf_alt_def
-      apply (subst bind_commute_spmf)
-      apply (intro
-        Utils_SPMF_Relational.seq'[where S = \<open>(=)\<close>]
-        Utils_SPMF_Relational.if_then_else
-        Utils_SPMF_Relational.seq'[where S = \<open>curry snd\<close>])
-      by (auto intro: Utils_SPMF_Hoare.seq' Utils_SPMF_Hoare.hoare_tripleI)
-
-    with SPMF.fundamental_lemma[
-      where p = \<open>p \<bind> ?go_with_flag f\<close>, where q = \<open>p \<bind> ?go_with_flag f'\<close>,
-      where A = \<open>P <<< snd\<close>, where B = \<open>P <<< snd\<close>,
-      where ?bad1.0 = fst, where ?bad2.0 = fst]
-    show ?thesis
-      by (fastforce
-        intro: rel_spmf_mono
-        simp add: Utils_SPMF_Relational.relational_hoare_triple_def)
-  qed
-
-  also have \<open>\<dots> \<le> \<P>(x in measure_spmf p. cond x)\<close>
-  proof -
-    have \<open>\<turnstile>spmf
-      \<lbrace>\<lblot>\<lblot>True\<rblot>\<rblot>\<rbrace>
-      \<langle>?kleisli_spmf_p (?go_with_flag f) | ?kleisli_spmf_p return_spmf\<rangle>
-      \<lbrace>(\<lambda> (flag, _) x'. flag \<longleftrightarrow> cond x')\<rbrace>\<close>
-      unfolding pair_spmf_alt_def
-      by (fastforce intro:
-        Utils_SPMF_Relational.seq[where S = \<open>(=)\<close>]
-        Utils_SPMF_Hoare.if_then_else Utils_SPMF_Hoare.seq'
-        Utils_SPMF_Hoare.postcond_true)
-
-    then show ?thesis
-      by (auto
-        dest: rel_spmf_measureD[where A = \<open>{x. fst x}\<close>]
-        simp add: Utils_SPMF_Relational.relational_hoare_triple_def)
-  qed
-
-  finally show ?thesis .
-qed
-
-lemma
-  assumes [simp] :
-    \<open>\<And> x. lossless_spmf (body x)\<close>
-    \<open>\<And> x. lossless_spmf (loop_spmf.while cond body x)\<close>
-  defines [simp] :
-    \<open>while_1 \<equiv> \<lambda> cond body x. if cond x then body x else return_spmf x\<close>
-  shows
-    \<open>\<bar>\<P>(x in measure_spmf <| p \<bind> while_1 cond body. P x)
-      - \<P>(x in measure_spmf <| p \<bind> loop_spmf.while cond body. P x)\<bar>
-    \<le> \<P>(x in measure_spmf p. cond x)\<close>
-  using aux'[
-    where f' = \<open>body >=> loop_spmf.while cond body\<close>,
-    where g = return_spmf, where cond = cond]
-  by (simp add: loop_spmf.while.simps[symmetric])
-
-(* Old, deprecated experiments below. *)
-
-lemma
-  fixes cond g
-  assumes
-    \<open>\<And> x. lossless_spmf (body x)\<close>
-    \<open>\<And> x. lossless_spmf (loop_spmf.while cond body x)\<close>
-  shows
-    \<open>\<bar>\<P>(x in measure_spmf <| do {x \<leftarrow> p; if cond x then body x else return_spmf x}.
-      P x)
-      - \<P>(x in measure_spmf <| bind_pmf p <| loop_spmf.while cond body. P x)\<bar>
-    \<le> \<P>(x in p. cond x)\<close>
-    (is
-      \<open>\<bar>\<P>(x in measure_spmf <| bind_pmf _ <| ?if. _)
-        - ?prob (loop_spmf.while _ _)\<bar>
-      \<le> ?R\<close>)
-proof -
-  let ?bind_spmf_p = \<open>(>=>) \<lblot>spmf_of_pmf p\<rblot>\<close>
-
-  let ?if_with_flag = \<open>\<lambda> x. pair_spmf (?if x) (return_spmf <| cond x)\<close>
-
-  let ?cond_with_flag = \<open>\<lambda> (x, _). cond x\<close>
-  let ?body_with_flag = \<open>\<lambda> (x, _). pair_spmf (body x) (return_spmf True)\<close>
-  let ?while_with_flag = \<open>\<lambda> flag x.
-    loop_spmf.while ?cond_with_flag ?body_with_flag (x, flag)\<close>
-
-  have while_with_flag_eq :
-    \<open>?while_with_flag flag x = (
-      if cond x
-      then pair_spmf (loop_spmf.while cond body x) (return_spmf True)
-      else return_spmf (x, flag))\<close> for flag x
-    apply (auto simp add: loop_spmf.while_simps pair_spmf_alt_def)
-    apply (intro bind_spmf_cong)
-    apply blast
-
-    (* To show that 2 while loops are equal, we appeal to their domain-theoretic
-    denotational semantics as least fixed points of transfinite iteration
-    sequences, and show, via transfinite induction, that they are upper bounds
-    of each other's sequences.
-
-    TODO: Try to derive a relational Hoare logic proof rule that provides a
-    simpler API by abstracting away all this domain-theoretic fiddling.
-    For reference, see ch5 of http://publications.rwth-aachen.de/record/814578/files/814578.pdf *)
-    apply (intro spmf.leq_antisym)
-    subgoal for x'
-      apply (induction arbitrary: flag x x' rule: loop_spmf.while_fixp_induct[where guard = \<open>\<lambda> (x, _). cond x\<close>])
-      by (auto
-        intro!: ord_spmf_bind_reflI
-        simp add: map_spmf_bind_spmf bind_map_spmf pair_spmf_alt_def loop_spmf.while_simps)
-
-    subgoal for x'
-      apply (induction arbitrary: flag x x' rule: loop_spmf.while_fixp_induct[where guard = cond])
-      by (auto
-        intro: ord_spmf_bind_reflI
-        simp add: map_spmf_bind_spmf bind_map_spmf pair_spmf_alt_def loop_spmf.while_simps)
-    done
-
-  with assms have \<open>lossless_spmf (?while_with_flag flag x)\<close> for flag x
-    by (simp add: pair_spmf_return_spmf2)
-
-  then have \<open>\<turnstile>spmf
-    \<lbrace>\<lblot>\<lblot>True\<rblot>\<rblot>\<rbrace>
-    \<langle>?bind_spmf_p ?if_with_flag | ?bind_spmf_p (?while_with_flag False)\<rangle>
-    \<lbrace>(\<lambda> (y, flag) (y', flag'). (flag \<longleftrightarrow> flag') \<and> (\<not> flag \<longrightarrow> y = y'))\<rbrace>\<close>
-    apply (intro Utils_SPMF_Relational.seq'[where S = \<open>(=)\<close>])
-    apply (simp add: Utils_SPMF_Relational.relational_hoare_triple_def spmf_rel_eq)
-    unfolding pair_spmf_alt_def
-    apply (simp add: if_distrib if_distribR loop_spmf.while.simps)
-    apply (intro Utils_SPMF_Relational.if_then_else)
-    apply blast
-    apply (intro Utils_SPMF_Relational.seq'[where S = \<open>\<lambda> x (x', flag). flag\<close>])
-    apply (simp add: Utils_SPMF_Relational.relational_hoare_triple_def)
-    apply (metis (no_types, lifting) bind_return_spmf case_prodI option.rel_inject(2) rel_pmf_return_pmfI rel_spmf_bind_reflI)
-    subgoal
-      apply (subst Utils_SPMF_Relational.skip_left')
-      apply (smt (verit, del_insts) case_prodE loop_spmf.while.simps lossless_return_spmf split_conv)
-      by (auto
-        intro!:
-          Utils_SPMF_Hoare.while Utils_SPMF_Hoare.seq'
-          Utils_SPMF_Hoare.postcond_true
-        simp add: case_prod_beta')
-    by (simp add: Utils_SPMF_Relational.relational_hoare_triple_def)
-
-  with SPMF.fundamental_lemma[
-    where p = \<open>p \<bind> ?if_with_flag\<close>,
-    where q = \<open>p \<bind> (?while_with_flag False)\<close>,
-    where A = \<open>P <<< fst\<close>, where B = \<open>P <<< fst\<close>,
-    of snd snd]
-  have
-    \<open>\<bar>\<P>(x in measure_spmf <| p \<bind> ?if_with_flag. P (fst x))
-      - \<P>(x in measure_spmf <| p \<bind> (?while_with_flag False). P (fst x))\<bar>
-    \<le> \<P>(x in measure_spmf <| p \<bind> ?if_with_flag. snd x)\<close>
-    by (fastforce
-      intro: rel_spmf_mono
-      simp add:
-        Utils_SPMF_Relational.relational_hoare_triple_def space_measure_spmf)
-
-  also have \<open>\<dots> \<le> ?R\<close>
-  proof -
-    from assms have \<open>\<turnstile>spmf
-      \<lbrace>\<lblot>\<lblot>True\<rblot>\<rblot>\<rbrace>
-      \<langle>?bind_spmf_p ?if_with_flag | ?bind_spmf_p return_spmf\<rangle>
-      \<lbrace>(\<lambda> (_, flag) x'. flag \<longleftrightarrow> cond x')\<rbrace>\<close>
-      unfolding pair_spmf_alt_def
-      apply (intro Utils_SPMF_Relational.seq[where S = \<open>(=)\<close>])
-      apply (simp add: Utils_SPMF_Relational.relational_hoare_triple_def spmf_rel_eq) 
-      by (auto intro: Utils_SPMF_Hoare.seq' Utils_SPMF_Hoare.postcond_true)
-
-    then show ?thesis
-      by (auto
-        dest: rel_spmf_measureD[where A = \<open>{x. snd x}\<close>]
-        simp add: Utils_SPMF_Relational.relational_hoare_triple_def space_measure_spmf)
-  qed
-
-  finally show ?thesis
-    apply (simp add: space_measure_spmf while_with_flag_eq)
-    using measure_map_spmf[of fst, where A = \<open>{x. P x}\<close>, simplified vimage_def, simplified]
-    by (smt (verit, best) bind_pmf_cong loop_spmf.while_simps(2) map_bind_pmf map_fst_pair_spmf pair_spmf_return_spmf scale_spmf_eq_same weight_return_spmf)
-qed
-
-(* lemma
-  assumes \<open>state ok\<close>
-  shows \<open>prob_fail (step_while x state) \<le> prob_fail (step x state)\<close>
-proof -
-  have \<open>\<turnstile>pmf
-    \<lbrakk>(\<lambda> state state'. state = state' \<and> (state ok))\<rbrakk>
-    \<langle>step x | step_while x\<rangle>
-    \<lbrakk>ord_option (=)\<rbrakk>\<close>
-    (is \<open>\<turnstile>pmf \<lbrakk>?R\<rbrakk> \<langle>_ | _ \<rangle> \<lbrakk>_\<rbrakk>\<close>)
-    unfolding
-      step_def step_while_def well_formed_state_def Let_def
-      Set.filter_def Set.remove_def 
-    apply (rule Utils_PMF_Relational.seq'[where S = \<open>(=)\<close>])
-    apply (simp add: Utils_PMF_Relational.relational_hoare_triple_def pmf.rel_refl)
-    apply (subst aux)
-    apply (simp_all add: card_insert_if le_diff_conv)
-    by (fastforce
-      intro: Utils_PMF_Relational.if_then_else Utils_PMF_Relational.seq'[where S = \<open>(=)\<close>]
-      simp add: aux Set.filter_def fail_spmf_def Utils_PMF_Relational.relational_hoare_triple_def pmf.rel_refl)
-
-  with assms show ?thesis
-    by (blast intro: prob_fail_le_of_relational_hoare_triple)
-qed *)
 
 end
 
