isabelle/Utils/SPMF/Utils_SPMF_Relational.thy
@@ -254,4 +254,232 @@ proof -
       Utils_PMF_Relational.relational_hoare_triple_def)
 qed
 
+text
+  \<open>If 2 probabilistic if-then-else expressions differ in only one branch of
+  computation, the total variation metric between their output distributions
+  is bounded by the probability that their guard condition evaluates such that
+  that branch of computation is taken.
+
+  This generalises and captures the essence behind bounding the distance between
+  running a while loop for only 1 iteration vs running it for \<ge> 1 iterations.
+
+  The proof of this result utilises the fundamental lemma for spmfs, along with
+  automation provided by our probabilistic relational Hoare logic for spmfs.
+
+  Note that the lossless assumptions are there because the proof uses
+  `pair_spmf` to "pair" the original function with a boolean flag indicating
+  if the condition evaluated to true or not. This is in turned used alongside
+  the fundamental lemma.\<close>
+lemma measure_spmf_dist_ite_le :
+  fixes cond g and f f' :: \<open>'a \<Rightarrow> 'a spmf\<close>
+  assumes [simp] :
+    \<open>\<And> x. lossless_spmf (f x)\<close>
+    \<open>\<And> x. lossless_spmf (f' x)\<close>
+    \<open>\<And> x. lossless_spmf (g x)\<close>
+  defines [simp] : \<open>go \<equiv> \<lambda> f x. if cond x then f x else g x\<close>
+  shows
+    \<open>\<bar>\<P>(x in measure_spmf <| p \<bind> go f. P x)
+      - \<P>(x in measure_spmf <| p \<bind> go f'. P x)\<bar>
+    \<le> \<P>(x in measure_spmf p. cond x)\<close>
+    (is \<open>?L \<le> _\<close>)
+proof -
+  let ?kleisli_spmf_p = \<open>(>=>) \<lblot>p\<rblot>\<close>
+  let ?go_with_flag = \<open>\<lambda> f x.
+    if cond x
+    then pair_spmf (return_spmf True) (f x)
+    else pair_spmf (return_spmf False) (g x)\<close>
+
+  note [simp] = space_measure_spmf
+
+  have \<open>?L =
+    \<bar>\<P>(x in measure_spmf <| p \<bind> ?go_with_flag f. P (snd x))
+      - \<P>(x in measure_spmf <| p \<bind> ?go_with_flag f'. P (snd x))\<bar>\<close>
+    apply (simp add:
+      if_distrib map_spmf_bind_spmf comp_def
+      measure_map_spmf[
+        of snd, where A = \<open>{x. P x}\<close>,
+        simplified vimage_def, simplified, symmetric])
+    unfolding map_snd_pair_spmf weight_return_spmf scale_spmf_1 ..
+
+  also have \<open>\<dots> \<le> \<P>(x in measure_spmf <| p \<bind> ?go_with_flag f. fst x)\<close>
+  proof -
+    have \<open>\<turnstile>spmf
+      \<lbrace>\<lblot>\<lblot>True\<rblot>\<rblot>\<rbrace>
+      \<langle>?kleisli_spmf_p (?go_with_flag f) | ?kleisli_spmf_p (?go_with_flag f')\<rangle>
+      \<lbrace>(\<lambda> (flag, y) (flag', y'). (flag \<longleftrightarrow> flag') \<and> (\<not> flag \<longrightarrow> y = y'))\<rbrace>\<close>
+      unfolding pair_spmf_alt_def
+      apply (subst bind_commute_spmf)
+      apply (intro
+        Utils_SPMF_Relational.seq'[where S = \<open>(=)\<close>]
+        Utils_SPMF_Relational.if_then_else
+        Utils_SPMF_Relational.seq'[where S = \<open>curry snd\<close>])
+      by (auto intro: Utils_SPMF_Hoare.seq' Utils_SPMF_Hoare.hoare_tripleI)
+
+    with SPMF.fundamental_lemma[
+      where p = \<open>p \<bind> ?go_with_flag f\<close>, where q = \<open>p \<bind> ?go_with_flag f'\<close>,
+      where A = \<open>P <<< snd\<close>, where B = \<open>P <<< snd\<close>,
+      where ?bad1.0 = fst, where ?bad2.0 = fst]
+    show ?thesis
+      by (fastforce
+        intro: rel_spmf_mono
+        simp add: Utils_SPMF_Relational.relational_hoare_triple_def)
+  qed
+
+  also have \<open>\<dots> \<le> \<P>(x in measure_spmf p. cond x)\<close>
+  proof -
+    have \<open>\<turnstile>spmf
+      \<lbrace>\<lblot>\<lblot>True\<rblot>\<rblot>\<rbrace>
+      \<langle>?kleisli_spmf_p (?go_with_flag f) | ?kleisli_spmf_p return_spmf\<rangle>
+      \<lbrace>(\<lambda> (flag, _) x'. flag \<longleftrightarrow> cond x')\<rbrace>\<close>
+      unfolding pair_spmf_alt_def
+      by (fastforce intro:
+        Utils_SPMF_Relational.seq[where S = \<open>(=)\<close>]
+        Utils_SPMF_Hoare.if_then_else Utils_SPMF_Hoare.seq'
+        Utils_SPMF_Hoare.postcond_true)
+
+    then show ?thesis
+      by (auto
+        dest: rel_spmf_measureD[where A = \<open>{x. fst x}\<close>]
+        simp add: Utils_SPMF_Relational.relational_hoare_triple_def)
+  qed
+
+  finally show ?thesis .
+qed
+
+lemma measure_spmf_dist_ite_while_le :
+  assumes [simp] :
+    \<open>\<And> x. lossless_spmf (body x)\<close>
+    \<open>\<And> x. lossless_spmf (loop_spmf.while cond body x)\<close>
+  defines [simp] :
+    \<open>while1 \<equiv> \<lambda> cond body x. if cond x then body x else return_spmf x\<close>
+  shows
+    \<open>\<bar>\<P>(x in measure_spmf <| p \<bind> while1 cond body. P x)
+      - \<P>(x in measure_spmf <| p \<bind> loop_spmf.while cond body. P x)\<bar>
+    \<le> \<P>(x in measure_spmf p. cond x)\<close>
+  using measure_spmf_dist_ite_le[
+    where f' = \<open>body >=> loop_spmf.while cond body\<close>,
+    where g = return_spmf, where cond = cond]
+  by (simp add: loop_spmf.while.simps[symmetric])
+
+(* Old, deprecated experiments below. *)
+
+lemma
+  fixes cond g
+  assumes
+    \<open>\<And> x. lossless_spmf (body x)\<close>
+    \<open>\<And> x. lossless_spmf (loop_spmf.while cond body x)\<close>
+  shows
+    \<open>\<bar>\<P>(x in measure_spmf <| do {x \<leftarrow> p; if cond x then body x else return_spmf x}.
+      P x)
+      - \<P>(x in measure_spmf <| bind_pmf p <| loop_spmf.while cond body. P x)\<bar>
+    \<le> \<P>(x in p. cond x)\<close>
+    (is
+      \<open>\<bar>\<P>(x in measure_spmf <| bind_pmf _ <| ?if. _)
+        - ?prob (loop_spmf.while _ _)\<bar>
+      \<le> ?R\<close>)
+proof -
+  let ?bind_spmf_p = \<open>(>=>) \<lblot>spmf_of_pmf p\<rblot>\<close>
+
+  let ?if_with_flag = \<open>\<lambda> x. pair_spmf (?if x) (return_spmf <| cond x)\<close>
+
+  let ?cond_with_flag = \<open>\<lambda> (x, _). cond x\<close>
+  let ?body_with_flag = \<open>\<lambda> (x, _). pair_spmf (body x) (return_spmf True)\<close>
+  let ?while_with_flag = \<open>\<lambda> flag x.
+    loop_spmf.while ?cond_with_flag ?body_with_flag (x, flag)\<close>
+
+  have while_with_flag_eq :
+    \<open>?while_with_flag flag x = (
+      if cond x
+      then pair_spmf (loop_spmf.while cond body x) (return_spmf True)
+      else return_spmf (x, flag))\<close> for flag x
+    apply (auto simp add: loop_spmf.while_simps pair_spmf_alt_def)
+    apply (intro bind_spmf_cong)
+    apply blast
+
+    (* To show that 2 while loops are equal, we appeal to their domain-theoretic
+    denotational semantics as least fixed points of transfinite iteration
+    sequences, and show, via transfinite induction, that they are upper bounds
+    of each other's sequences.
+
+    TODO: Try to derive a relational Hoare logic proof rule that provides a
+    simpler API by abstracting away all this domain-theoretic fiddling.
+    For reference, see ch5 of http://publications.rwth-aachen.de/record/814578/files/814578.pdf *)
+    apply (intro spmf.leq_antisym)
+    subgoal for x'
+      apply (induction arbitrary: flag x x' rule: loop_spmf.while_fixp_induct[where guard = \<open>\<lambda> (x, _). cond x\<close>])
+      by (auto
+        intro!: ord_spmf_bind_reflI
+        simp add: map_spmf_bind_spmf bind_map_spmf pair_spmf_alt_def loop_spmf.while_simps)
+
+    subgoal for x'
+      apply (induction arbitrary: flag x x' rule: loop_spmf.while_fixp_induct[where guard = cond])
+      by (auto
+        intro: ord_spmf_bind_reflI
+        simp add: map_spmf_bind_spmf bind_map_spmf pair_spmf_alt_def loop_spmf.while_simps)
+    done
+
+  with assms have \<open>lossless_spmf (?while_with_flag flag x)\<close> for flag x
+    by (simp add: pair_spmf_return_spmf2)
+
+  then have \<open>\<turnstile>spmf
+    \<lbrace>\<lblot>\<lblot>True\<rblot>\<rblot>\<rbrace>
+    \<langle>?bind_spmf_p ?if_with_flag | ?bind_spmf_p (?while_with_flag False)\<rangle>
+    \<lbrace>(\<lambda> (y, flag) (y', flag'). (flag \<longleftrightarrow> flag') \<and> (\<not> flag \<longrightarrow> y = y'))\<rbrace>\<close>
+    apply (intro Utils_SPMF_Relational.seq'[where S = \<open>(=)\<close>])
+    apply (simp add: Utils_SPMF_Relational.relational_hoare_triple_def spmf_rel_eq)
+    unfolding pair_spmf_alt_def
+    apply (simp add: if_distrib if_distribR loop_spmf.while.simps)
+    apply (intro Utils_SPMF_Relational.if_then_else)
+    apply blast
+    apply (intro Utils_SPMF_Relational.seq'[where S = \<open>\<lambda> x (x', flag). flag\<close>])
+    apply (simp add: Utils_SPMF_Relational.relational_hoare_triple_def)
+    apply (metis (no_types, lifting) bind_return_spmf case_prodI option.rel_inject(2) rel_pmf_return_pmfI rel_spmf_bind_reflI)
+    subgoal
+      apply (subst Utils_SPMF_Relational.skip_left')
+      apply (smt (verit, del_insts) case_prodE loop_spmf.while.simps lossless_return_spmf split_conv)
+      by (auto
+        intro!:
+          Utils_SPMF_Hoare.while Utils_SPMF_Hoare.seq'
+          Utils_SPMF_Hoare.postcond_true
+        simp add: case_prod_beta')
+    by (simp add: Utils_SPMF_Relational.relational_hoare_triple_def)
+
+  with SPMF.fundamental_lemma[
+    where p = \<open>p \<bind> ?if_with_flag\<close>,
+    where q = \<open>p \<bind> (?while_with_flag False)\<close>,
+    where A = \<open>P <<< fst\<close>, where B = \<open>P <<< fst\<close>,
+    of snd snd]
+  have
+    \<open>\<bar>\<P>(x in measure_spmf <| p \<bind> ?if_with_flag. P (fst x))
+      - \<P>(x in measure_spmf <| p \<bind> (?while_with_flag False). P (fst x))\<bar>
+    \<le> \<P>(x in measure_spmf <| p \<bind> ?if_with_flag. snd x)\<close>
+    by (fastforce
+      intro: rel_spmf_mono
+      simp add:
+        Utils_SPMF_Relational.relational_hoare_triple_def space_measure_spmf)
+
+  also have \<open>\<dots> \<le> ?R\<close>
+  proof -
+    from assms have \<open>\<turnstile>spmf
+      \<lbrace>\<lblot>\<lblot>True\<rblot>\<rblot>\<rbrace>
+      \<langle>?bind_spmf_p ?if_with_flag | ?bind_spmf_p return_spmf\<rangle>
+      \<lbrace>(\<lambda> (_, flag) x'. flag \<longleftrightarrow> cond x')\<rbrace>\<close>
+      unfolding pair_spmf_alt_def
+      apply (intro Utils_SPMF_Relational.seq[where S = \<open>(=)\<close>])
+      apply (simp add: Utils_SPMF_Relational.relational_hoare_triple_def spmf_rel_eq) 
+      by (auto intro: Utils_SPMF_Hoare.seq' Utils_SPMF_Hoare.postcond_true)
+
+    then show ?thesis
+      by (auto
+        dest: rel_spmf_measureD[where A = \<open>{x. snd x}\<close>]
+        simp add: Utils_SPMF_Relational.relational_hoare_triple_def space_measure_spmf)
+  qed
+
+  finally show ?thesis
+    apply (simp add: space_measure_spmf while_with_flag_eq)
+    using measure_map_spmf[of fst, where A = \<open>{x. P x}\<close>, simplified vimage_def, simplified]
+    by (smt (verit, best) bind_pmf_cong loop_spmf.while_simps(2) map_bind_pmf map_fst_pair_spmf pair_spmf_return_spmf scale_spmf_eq_same weight_return_spmf)
+qed
+
+
 end
